Tweaks

src/QueueInterface.v
@@ -13,102 +13,87 @@ Definition a := nat.
 
 Inductive Op : Type :=
 | Empty
-| Push
+| Push (x : a)
 | Pop
-| New (x : a)  (* As argument to push *)
 .
 
-Inductive Value : Type :=
-| Q (q : Queue a)
-| E (x : a)
-.
-
-Definition queue_eval_op (o : Op) (vs : list Value) : list Value :=
+Definition queue_eval_op (o : Op) (vs : list (Queue a)) : list (Queue a) :=
   match o, vs with
-  | Empty, _ => [Q empty]
-  | Push, Q q :: E x :: _ => [Q (push q x)]
-  | Pop, Q q :: _ =>
+  | Empty, _ => [empty]
+  | Push x, q :: _ => [push q x]
+  | Pop, q :: _ =>
     match pop q with
     | None => []
-    | Some (x, q) => [E x; Q q]
+    | Some (x, q) => [q]
     end
-  | New x, _ => [E x]
   | _, _ => []
   end.
 
-#[global] Instance queue_pure_impl : PureImpl Op Value := queue_eval_op.
+#[global] Instance PureImpl_Queue : PureImpl Op (Queue a) := queue_eval_op.
 
-Definition cost (_ : Op) (_ : list Value) : nat := 7.
+#[global] Instance CostSpec_Queue : CostSpec Op (Queue a) :=
+  fun o vs =>
+    match o with
+    | Empty => 1
+    | Push _ => 1
+    | Pop => 1
+    end.
 
-Inductive ValueA : Type :=
-| QA (q : T (QueueA a))
-| EA (x : T a)
-.
+Definition cost (_ : Op) (_ : list (Queue a)) : nat := 7.
 
-Definition queue_exec_op (o : Op) (vs : list ValueA) : M (list ValueA) :=
+Definition TQueueA := T (QueueA a).
+
+Definition queue_exec_op (o : Op) (vs : list TQueueA) : M (list TQueueA) :=
   match o, vs with
-  | Empty, _ => let~ q := emptyA in ret [QA q]
-  | Push, QA q :: EA x :: _ => let~ q' := pushA q x in ret [QA q']
-  | Pop, QA q :: _ =>
+  | Empty, _ => let~ q := emptyA in ret [q]
+  | Push x, q :: _ => let~ q' := pushA q (Thunk x) in ret [q']
+  | Pop, q :: _ =>
     let! pop_q := popA q in
     match pop_q with
     | None => ret []
-    | Some (x, q) => ret [EA x; QA q]
+    | Some (x, q) => ret [q]
     end
-  | New x, _ => ret [EA (Core.Thunk x)]
   | _, _ => ret []
   end.
 
-#[global] Instance queue_cv_impl : CvImpl Op ValueA := queue_exec_op.
-
-#[global] Instance Exact_Value : Exact Value ValueA := fun v =>
-  match v with
-  | Q q => QA (exact q)
-  | E x => EA (exact x)
-  end.
-
-#[global] Instance Lub_ValueA : Lub ValueA := fun v v' =>
-  match v, v' with
-  | QA q, QA q' => QA (lub q q')
-  | EA x, EA x' => EA (lub x x')
-  | _, _ => EA Undefined
-  end.
-
-Inductive LessDefined_ValueA : LessDefined ValueA :=
-| less_defined_QA {q q'} : q `less_defined` q' -> LessDefined_ValueA (QA q) (QA q')
-| less_defined_EA {x x'} : x `less_defined` x' -> LessDefined_ValueA (EA x) (EA x')
-.
-
-#[local] Existing Instance LessDefined_ValueA.
-
-#[local] Instance PreOrder_LessDefined_ValueA : PreOrder (less_defined (a := ValueA)).
-Admitted.
-
-#[local] Instance LubLaw_ValueA : LubLaw ValueA.
-Admitted.
+#[global] Instance CvImpl_Queue : CvImpl Op TQueueA := queue_exec_op.
 
 #[local] Instance exec_op_mon (o : Op) :
   Morphisms.Proper (Morphisms.respectful less_defined less_defined)
-    (exec_op (op := Op) (valueA := ValueA) o).
+    (exec_op (op := Op) (valueA := TQueueA) o).
 Proof.
   intros ? ? E. destruct o; cbn.
   - reflexivity.
   - destruct E as [ | ? ? ? ? E1 E].
     + reflexivity.
-    + destruct E1; [ | reflexivity ].
-      destruct E as [ | ? ? ? ? E2 E]; [ reflexivity | ].
-      destruct E2;  [ reflexivity | ].
-      apply bind_mon; [ apply thunk_mon, pushA_mon; auto | intros; apply ret_mon ].
-      constructor; constructor. auto.
+    + apply bind_mon; [ apply thunk_mon, pushA_mon; reflexivity + auto | intros; apply ret_mon ].
+      constructor; constructor + auto.
   - destruct E as [ | ? ? ? ? E1 E ]; [ reflexivity | ].
-    destruct E1; [ | reflexivity ].
     apply bind_mon; [ apply popA_mon; auto | intros ? ? []; [ reflexivity | ] ].
-    destruct H0. destruct x0, y.
-    apply ret_mon. repeat (assumption + constructor).
-  - apply ret_mon. repeat constructor.
+    destruct x1, y0.
+    apply ret_mon. repeat (constructor + apply H).
 Qed.
 
-#[global] Instance ImplApprox_Queue : ImplApprox Op Value ValueA.
+#[global] Instance ImplApprox_Queue : ImplApprox Op (Queue a) TQueueA.
 Proof.
   econstructor; try typeclasses eauto.
+Defined.
+
+(* "debt" in BankersQueue *)
+Definition potential : TQueueA -> nat := fun Tq =>
+  match Tq with
+  | Undefined => 0
+  | Thunk qA => 2 * sizeX 0 (frontA qA) - 2 * nbackA qA
+  end.
+
+Lemma potential_lub_QueueA : forall qA qA' : TQueueA, cobounded qA qA' -> potential (lub qA qA') <= potential qA + potential qA'.
+Proof.
+  unfold TQueueA. apply @LubDebt_T, @LubDebt_QueueA.
 Qed.
+
+#[global] Instance HasAmortizedCost_Queue : HasAmortizedCost Op (Queue a) TQueueA.
+Proof.
+  apply Build_HasAmortizedCost with (potential := potential).
+  - exact @potential_lub_QueueA.
+  - admit.
+Admitted.
